proof/spec/Wots.ec
@@ -5,14 +5,13 @@ require (*  *) Subtype.
 
 from Jasmin require import JModel.
 
-require import Notation Address Primitives.
+require import Params Notation Address Primitives.
 
 import DList.
 import NBytes.
 
-(* sk = u8[XMSS_WOTS_LEN * XMSS_N] = u8[XMSS_WOTS_LEN][XMSS_N] *)
-(* LEN elements, each with N-byte strings *)
-(* XMSS_N is determined by the cryptographic hash functions we use *)
+(**********************************************************************************************************************)
+
 clone import Subtype as LEN_N with 
    type T = nbytes list,
    op P = fun l => size l = len
@@ -20,7 +19,6 @@ clone import Subtype as LEN_N with
    proof inhabited by (exists (nseq len (nseq n W8.zero));smt(size_nseq ge0_len))
    proof *.
 
-axiom ge0_len1 : 0 <= len1.
 
 clone import Subtype as LEN1 with 
    type T = byte list,
@@ -29,20 +27,24 @@ clone import Subtype as LEN1 with
    proof inhabited by (exists (nseq len1 W8.zero);smt(size_nseq ge0_len1))
    proof *.
 
+(**********************************************************************************************************************)
 
 type wots_message = nbytes.
 type wots_message_base_w = len1_bytes.
+type wots_signature = len_n_bytes.
 type wots_pk = len_n_bytes.
 type wots_sk = len_n_bytes.
 type wots_keypair = wots_pk * wots_sk.
-type wots_signature = len_n_bytes.
 
-op from_int_list (x : int list) : byte list = map W8.of_int x.
-op W32_of_W8 (x : W8.t) : W32.t = W32.of_int (W8.to_uint x).
+(**********************************************************************************************************************)
 
-op prf_keygen : nbytes -> nbytes -> nbytes.
+(* For pseudorandomly generate a WOTS private key from a secret seed *)
+op PRF_KEYGEN (sk_seed : nbytes, address : adrs, seed : nbytes) : nbytes.
+
+(**********************************************************************************************************************)
 
 module WOTS = {
+  (* In practise, we generate the private key from a secret seed *)
   proc genSK() : wots_sk = {
     var sk : wots_sk <- nseq len (nseq n W8.zero);
     var sk_i : nbytes;
@@ -56,30 +58,35 @@ module WOTS = {
 
     return sk;
   }
-  
+
   (* 
   Pseudorandom Key Generation [Section 3.1.7. of the RFC]
 
-  During key generation, a uniformly random n-byte string S is
-  sampled from a secure source of randomness. This string S is stored
-  as private key. The private key elements are computed as sk[i] =
-  PRF(S, toByte(i, 32)) whenever needed. Please note that this seed S
-  MUST be different from the seed SEED used to randomize the hash
-  function calls. Also, this seed S MUST be kept secret. The seed S
-  MUST NOT be a low entropy, human-memorable value since private key
-  elements are derived from S deterministically and their
-  confidentiality is security-critical.
+    During key generation, a uniformly random n-byte string S is
+    sampled from a secure source of randomness. This string S is stored
+    as private key. The private key elements are computed as sk[i] =
+    PRF(S, toByte(i, 32)) whenever needed. Please note that this seed S
+    MUST be different from the seed SEED used to randomize the hash
+    function calls. Also, this seed S MUST be kept secret. The seed S
+    MUST NOT be a low entropy, human-memorable value since private key
+    elements are derived from S deterministically and their
+    confidentiality is security-critical.
+
   *)
-  proc pseudorandom_genSK(s : nbytes) = {
-    var sk : wots_sk <- nseq len (nseq n W8.zero);
+  proc pseudorandom_genSK(sk_seed : nbytes, seed : nbytes, address : adrs) : wots_sk = {
+    var sk : wots_sk <- nseq len (nseq n witness);
     var sk_i : nbytes;
     var key : nbytes;
     var i : int;
     
+    address <- set_hash_addr address 0;
+    address <- set_key_and_mask address 0;
+
     i <- 0;
-    while (i < n) {
+    while (i < len) {
+      address <- set_chain_addr address i;
       key <- toByte (W32.of_int i) 32;
-      sk_i <- prf_keygen s key;
+      sk_i <- PRF_KEYGEN sk_seed address key;
       sk <- put sk i sk_i;
       i <- i + 1;
     }
@@ -87,6 +94,8 @@ module WOTS = {
     return sk;
   }
 
+  (* The len n-byte strings in the private key each define the start node for one hash chain. The public
+  key consists of the end nodes of these hash chains *)
   proc genPK(sk : wots_sk, _seed : seed, address : adrs) : wots_pk = {
     var pk : wots_pk <- nseq len (nseq n W8.zero);
     var i : int <- 0;
@@ -107,53 +116,60 @@ module WOTS = {
     var pk : wots_pk;
     var sk : wots_sk;
 
-    sk <@ pseudorandom_genSK(sk_seed);
+    sk <@ pseudorandom_genSK(sk_seed, _seed, address);
     pk <@ genPK(sk, _seed, address);
 
     return (pk, sk);
   }
 
-(*
-             +---------------------------------+
-             |                                 |
-             |           sig_ots[0]            |    n bytes
-             |                                 |
-             +---------------------------------+
-             |                                 |
-             ~              ....               ~
-             |                                 |
-             +---------------------------------+
-             |                                 |
-             |          sig_ots[len - 1]       |    n bytes
-             |                                 |
-             +---------------------------------+
-
-                              WOTS+ Signature
-*)
-
-  proc sign(m : wots_message, sk : wots_sk, _seed : seed, address : adrs) : wots_signature = {
-    var csum : W32.t <- W32.zero;
-    var m_i : W8.t;
-    var sig : wots_signature <- witness;
-    var sig_i : nbytes;
-    var sk_i : nbytes;
-    var msg_i : int;
-    var _m : int list;
+  proc checksum (m : int list) : W32.t = {
     var i : int <- 0;
+    var m_i : int <- witness;
+    var checksum : int <- 0;
+
+    while (i < len1) {
+      m_i <- nth witness m i;
+      checksum <- checksum + (w - 1) - m_i;
+      i <- i + 1;
+    }
+
+    return (W32.of_int checksum);
+  }
+
+  (*
+               +---------------------------------+
+               |                                 |
+               |           sig_ots[0]            |    n bytes
+               |                                 |
+               +---------------------------------+
+               |                                 |
+               ~              ....               ~
+               |                                 |
+               +---------------------------------+
+               |                                 |
+               |          sig_ots[len - 1]       |    n bytes
+               |                                 |
+               +---------------------------------+
+
+                                WOTS+ Signature
+  *)
+  proc sign(M : wots_message, sk : wots_sk, _seed : seed, address : adrs) : wots_signature = {
+    var csum : W32.t;
+    var msg : int list;
+    var msg_i : int;
+    var sk_i : nbytes;
     var len_2_bytes : int;
     var csum_bytes : byte list;
     var csum_base_w : int list;
+    var sig : wots_signature <- witness;
+    var sig_i : nbytes;
+    var i : int;
 
     (* Convert message to base w *)
-    _m <@ BaseW.base_w(m, len1);
-    m <- from_int_list _m;
+    msg <@ BaseW.base_w(M, len1);
 
     (* Compute checksum *)
-    while (i < len1) {
-      m_i <- nth witness m i;
-      csum <- csum + W32.of_int(w - 1) - (W32_of_W8 m_i);
-      i <- i + 1;
-    }
+    csum <@ checksum(msg);
 
     (* Convert checksum to base w *)
     csum <- csum `<<` W8.of_int (8 - ((ceil (len2%r * log2(w%r))) %% 8));
@@ -162,13 +178,13 @@ module WOTS = {
     (* msg = msg || base_w(toByte(csum, len_2_bytes), w, len_2); *)
     csum_bytes <- toByte csum len;
     csum_base_w <@ BaseW.base_w(csum_bytes, len_2_bytes);
-    m <- m ++ (from_int_list csum_base_w);
+    msg <- msg ++ csum_base_w;
 
     i <- 0;
     while (i < len) {
       address <- set_chain_addr address i;
+      msg_i <- nth witness msg i;
       sk_i <- nth witness sk i;
-      msg_i <- W8.to_uint (nth witness m i);
       sig_i <@ Chain.chain (sk_i, 0, msg_i, _seed, address);
       sig <- put sig i sig_i;
       i <- i + 1;
@@ -177,32 +193,23 @@ module WOTS = {
     return sig;
   }
 
-
-  (* Note: XMSS uses WOTS_pkFromSig to compute a public key value and
-     delays the comparison to a later point. *)
-  proc pkFromSig(m : wots_message, sig : wots_signature, _seed : seed, address : adrs) : wots_pk = {
+  proc pkFromSig(M : wots_message, sig : wots_signature, _seed : seed, address : adrs) : wots_pk = {
     var tmp_pk : wots_pk <- witness;
-    var csum : W32.t <- W32.zero;
-    var pk_i : nbytes;
-    var m_i : W8.t;
-    var _m : int list;
-    var i : int <- 0;
+    var csum : W32.t;
+    var msg : int list;
     var len_2_bytes : int;
-    var sig_i : nbytes;
-    var msg_i : int;
     var csum_bytes : byte list;
     var csum_base_w : int list;
+    var i : int;
+    var sig_i : nbytes;
+    var msg_i : int;
+    var pk_i : nbytes;
 
     (* Convert message to base w *)
-    _m <@ BaseW.base_w(m, len1);
-    m <- from_int_list _m;
+    msg <@ BaseW.base_w(M, len1);
 
     (* Compute checksum *)
-    while (i < len1) {
-      m_i <- nth witness m i;
-      csum <- csum + W32.of_int(w - 1) - (W32_of_W8 m_i);
-      i <- i + 1;
-    }
+    csum <@ checksum(msg);
 
     (* Convert checksum to base w *)
     csum <- csum `<<` W8.of_int (8 - ((ceil (len2%r * log2(w%r))) %% 8));
@@ -211,13 +218,13 @@ module WOTS = {
     (* msg = msg || base_w(toByte(csum, len_2_bytes), w, len_2); *)
     csum_bytes <- toByte csum len;
     csum_base_w <@ BaseW.base_w(csum_bytes, len_2_bytes);
-    m <- m ++ (from_int_list csum_base_w);
-
+    msg <- msg ++ csum_base_w;
+    
     i <- 0;
     while (i < len) {
       address <- set_chain_addr address i;
+      msg_i <- nth witness msg i;
       sig_i <- nth witness sig i;
-      msg_i <- W8.to_uint (nth witness m i);
       pk_i <@ Chain.chain (sig_i, msg_i, (w - 1 - msg_i), _seed, address);
       tmp_pk <- put tmp_pk i pk_i; 
       i <- i + 1;
@@ -233,18 +240,13 @@ module WOTS = {
   }
 }.
 
+(**********************************************************************************************************************)
+
 (* RFC - p 17
-Note that the checksum may reach a maximum integer value of len_1 * (w - 1) * 2^8 
-and therefore depends on the parameters n and w.
-
-
+Note that the checksum may reach a maximum integer value of len_1 * (w - 1) * 2^8.
 For the parameter sets specified in the RFC, a  32-bit unsigned integer is sufficient 
-to hold the checksum
- *)
-pred wots_checksum_pred (checksum : W32.t) =
-  W32.to_uint checksum <= len1 * (w - 2^8).
+to hold the checksum.
+*)
 
-(* ??? *)
-axiom wots_pseudorandom_keygen (s : nbytes) : 
-    equiv[WOTS.genSK ~ WOTS.pseudorandom_genSK : true ==> true].
-
+axiom checksum_max : hoare[WOTS.checksum : true ==> to_uint res <= len1 * (w - 1) * 2^8].
+axiom checksum_W32 : hoare[WOTS.checksum : true ==> to_uint res <= W32.max_uint].
