proof/correctness/Correctness_Wots.ec
@@ -3,13 +3,12 @@ pragma Goals : printall.
 
 require import AllCore List RealExp IntDiv.
 from Jasmin require import JModel.
-require import Notation Parameters Address Primitives Wots.
+require import Params Notation Parameters Address Primitives Wots.
 require import XMSS_IMPL XMSS_IMPL_PP Parameters.
-require import Generic Properties.
+require import Generic (* Properties *). 
 require import Array2 Array3 Array8 Array32 Array67 Array2144.
 
 lemma array3_list_put ['a] (x : 'a Array3.t) (v : 'a) (i : int) : put (to_list x) i v = to_list (x.[i <- v]) by admit.
-
 lemma array67_list_put ['a] (x : 'a Array67.t) (v : 'a) (i : int) : put (to_list x) i v = to_list (x.[i <- v]) by admit.
 
 lemma zero (x : int) :
@@ -121,6 +120,62 @@ smt. (* smt(@W64) fails *)
 smt(array67_list_put).
 qed.
 
+
+lemma base_w_correctness_67 (_out : W32.t Array67.t, _in_ : W8.t Array32.t) :
+    floor (log2 w%r) = XMSS_WOTS_LOG_W => 
+    equiv[M(Syscall).__base_w_67_32 ~ BaseW.base_w :
+      arg{1} = (_out, _in_) /\
+      arg{2} = (to_list _in_, 67) ==>
+        res{2} = map W32.to_uint (to_list res{1})].
+proof.
+move => logw.
+proc.
+auto => /> *.
+while (
+  outlen{2} = 67 /\
+  0 <= to_uint consumed{1} <= 67 /\
+  consumed{2} = to_uint consumed{1} /\
+  X{2} = to_list input{1} /\
+  to_uint bits{1} = bits{2} /\
+  ={total} /\
+  0 <= _in{2} <= 67 /\
+  W64.zero \ule in_0{1} /\ in_0{1} \ule W64.of_int 67 /\
+  _in{2} = to_uint in_0{1} /\
+  forall (k : int), (0 <= k < out{2}) => to_uint (output{1}.[k]) = nth witness base_w{2} k
+) ; last by admit.
+if ; last by admit.
+(* 1st subgoal of if *)
+auto => /> &1 &2 *. smt.
+(* 2nd subgoal of if *)
+auto => /> * ; do split.
+(* 1 *)
+smt(@W64).
+(* 2 *)
+smt(@W64).
+(* 3 *)
+smt.
+(* 4 *)
+rewrite logw => //.
+(* 5 *)
+smt().
+(* 6 *)
+admit.
+(* 7 *)
+admit.
+(* 8 *)
+admit.
+(* 9 *)
+admit.
+(* 10 *)
+move => ? . admit.
+(* 11 *)
+smt(@W64).
+(* 12 *)
+move => ? . admit.
+(* 3rd subgoal of if *)
+qed.
+
+
 (* We need to prove that (nth witness X{`&2} _in{`&2} `>>`  (of_int (bits{`&2} + 8 - floor (log2 w%r)))%W8) `&`  (of_int (w - 1))%W8))
 ((SHR_32 (zeroextu32 (nth witness X{`&2} (to_uint ((of_int _in{`&2}))%W64))) (truncateu8 ((of_int (bits{`&2} + 4)))%W64)).`6 `&` (of_int 15)%W32)) *)
 
@@ -131,64 +186,14 @@ lemma base_w_correctness (x_out : W32.t list, len_out : int, in_list : byte list
       equiv[BaseWGeneric.__base_w ~ BaseW.base_w :
         arg{1} = (x_out, W64.of_int len_out, in_list) /\
         arg{2} = (in_list, len_out) ==> 
-          res{1} = map W32.of_int res{2}].
+          res{2} = map W32.to_uint res{1}].
 proof.
-rewrite /XMSS_WOTS_W /XMSS_WOTS_LOG_W.
+rewrite /XMSS_WOTS_LEN /XMSS_WOTS_LEN2 /XMSS_WOTS_W /XMSS_WOTS_LOG_W.
 move => H.
 move: H => [#] len__out w_vals logw.
-proc ; inline.
-auto => /> *.
-while (
-  outlen{2} = len_out /\
-  outlen{1} = W64.of_int outlen{2} /\
-  consumed{1} = W64.of_int consumed{2} /\
-  input{1} = X{2} /\
-  bits{2} = to_uint bits{1} /\
-  ={total} /\
-  _in{2} = to_uint in_0{1} /\ 
-  to_uint in_0{1} + 1 < W64.max_uint /\
-  0 <= consumed{2} <= outlen{2} /\
-  0 <= _in{2} < outlen{2}  /\
-  forall (k : int), (0 <= k < consumed{2}) => to_uint (nth witness output{1} k) = nth witness base_w{2} k
-).
-(* ------------------------- first subgoal of while starts here ------------------------- *)
-if.
-(* 1st goal of if *)
-auto => /> &1 &2 *.
-smt(@W64).
-(* 2nd goal of if *)
-auto => /> &1 &2 *.
-do split.
-rewrite logw //=. (* 1st subgoal of split *)
-smt.
-admit. (* 2nd subgoal of split *)
-smt(). (* 3rd subgoal of split *)
-smt(). (* 4th subgoal of split *)
-smt(). (* 5th subgoal of split *)
-simplify.
-smt(). (* 6th subgoal of split *)
-smt. (* 9th *)
-(* 3rd subgoal of if *)
-auto => /> *.
-do split ; 2,3,4,6: by smt().
-(* 1 *) rewrite logw //=.
-(* 5 *) admit. (*`move => *. rewrite logw w_val /=. split. admit. admit. smt. *)
-(* 7 *) smt.
-(* ------------------------- second subgoal of while starts here ------------------------- *)
-auto => /> *.
-do split; 1,2: by smt().
-(* 3 *) smt.
-(* 4 *) smt.
-qed.
-
-
-lemma base_w_ll : islossless BaseWGeneric.__base_w.
-proof.
 proc.
-islossless.
-while (true) ((to_uint outlen) - (to_uint consumed)) ; last by auto => /> /#.
 auto => /> *.
-smt.
+admit.
 qed.
 
 (*********************************** EXPAND SEED ************************************************)
@@ -204,20 +209,54 @@ while (true) (8 - i1) ; last by skip ; auto => /> /#.
 auto => /> /#.
 while (true) (inlen - (to_uint i0)) => //=.
 auto => /> *.
-smt.
+admit.
 skip ; auto => /> *. 
-smt.
+admit.
+qed.
+
+lemma expand_seed_correctness (out : W8.t Array2144.t, _in : W8.t Array32.t, seed : W8.t Array32.t, address : W32.t Array8.t) :
+    n = XMSS_N =>
+    equiv[Mp(Syscall).__expand_seed ~ WOTS.pseudorandom_genSK :
+      arg{1} = (out, _in, seed, address) /\
+      arg{2} = to_list _in ==>
+      flatten(res{2}) = to_list res{1}.`1].
+proof. 
+rewrite /XMSS_N. move => H.
+proc ; inline => //=.
+auto => /> *.
+rewrite /XMSS_N.
+while (
+  n = XMSS_N /\
+  0 <= i{2} <= n /\
+  ={i}
+).
+admit.
+admit.
 qed.
 
 (****************************** GEN CHAIN ********************************************************)
 
-lemma wots_gen_chain_ll: islossless Mp(Syscall).__gen_chain_inplace.
-proof.
-proc ; inline => /=.
-islossless => //=.
-admit.
-qed.
+lemma chain_correctness (mem, _out : W8.t Array32.t, _in_ptr : W64.t, _start : W32.t,
+                         _steps : W32.t, seed : W8.t Array32.t, _address : W32.t Array8.t) :
+    n = XMSS_N => 
+    equiv [Mp(Syscall).__gen_chain ~ Chain.chain :
+      Glob.mem{1} = mem /\ Glob.mem{2} = mem /\
+      arg{1} = (_out, _in_ptr, _start, _steps, seed, address) /\
+      arg{2} = (mkseq (fun i => loadW8 mem (W64.to_uint (_in_ptr + (W64.of_int i))) n), 
+                to_uint _start, to_uint _steps, to_list seed, _address) =>
+        true].
 
+lemma chain_inplace (_out : W8.t Array32.t, _in_ptr : W64.t, _start:W32.t,
+                     _steps : W32.t, seed : W8.t Array32.t, address : W32.t Array8.t) :
+equiv [Mp(Syscall).__gen_chain ~ Mp(Syscall).__gen_chain_inplace :
+      ={Glob.mem} /\
+      arg{1} = (_out, _in_ptr, _start, _steps, seed, address) /\
+      arg{2} = (Array32.init (fun (i : int) => loadW8 Glob.mem{2} ((to_uint _in_ptr) + i)),
+                _start, _steps, seed, address) ==> true].
+proof.
+proc ; inline => //=.
+auto => /> *.
+admit.
 
 (***************************************************************************************)
 
@@ -265,7 +304,7 @@ proof. proc. while (true) (64 - (to_uint i)); by auto => /> * ; smt. qed.
 lemma wots_checksum_correctness (msg : W32.t Array67.t) :
     len1 = XMSS_WOTS_LEN1 => 
     w = XMSS_WOTS_W =>
-    equiv [Mp(Syscall).__csum ~ Checksum.checksum :
+    equiv [Mp(Syscall).__csum ~ WOTS.checksum :
       arg{1} = msg /\ arg{2} = to_list msg ==> to_uint res{1} = to_uint res{2}].
 proof.
 rewrite /XMSS_WOTS_LEN_1 /XMSS_WOTS_W ; move => ? ?.
