proof/correctness/Utils.ec
@@ -1,0 +1,5 @@
+pragma Goals : printall.
+
+require import AllCore List RealExp IntDiv.
+
+op drop_fst (). (* TODO: *)
