proof/extraction/XMSS_IMPL.ec
@@ -961,6 +961,21 @@ module M(SC:Syscall_t) = {
     return (out);
   }
   
+  proc __ull_to_bytes_32 (out:W8.t Array32.t, in_0:W64.t) : W8.t Array32.t = {
+    var aux: int;
+    
+    var i:int;
+    
+    aux <- (- 1);
+    i <- (32 - 1);
+    while (aux < i) {
+      out.[i] <- (truncateu8 in_0);
+      in_0 <- (in_0 `>>` (W8.of_int 8));
+      i <- i - 1;
+    }
+    return (out);
+  }
+  
   proc __ull_to_bytes_2 (out:W8.t Array2.t, in_0:W64.t) : W8.t Array2.t = {
     var aux: int;
     
@@ -983,21 +998,6 @@ module M(SC:Syscall_t) = {
     
     aux <- (- 1);
     i <- (4 - 1);
-    while (aux < i) {
-      out.[i] <- (truncateu8 in_0);
-      in_0 <- (in_0 `>>` (W8.of_int 8));
-      i <- i - 1;
-    }
-    return (out);
-  }
-  
-  proc __ull_to_bytes_32 (out:W8.t Array32.t, in_0:W64.t) : W8.t Array32.t = {
-    var aux: int;
-    
-    var i:int;
-    
-    aux <- (- 1);
-    i <- (32 - 1);
     while (aux < i) {
       out.[i] <- (truncateu8 in_0);
       in_0 <- (in_0 `>>` (W8.of_int 8));
@@ -1173,8 +1173,8 @@ module M(SC:Syscall_t) = {
     return ();
   }
   
-  proc __memcpy_u8u8_32_32 (out:W8.t Array32.t, offset:W64.t,
-                            in_0:W8.t Array32.t) : W8.t Array32.t * W64.t = {
+  proc __memcpy_u8u8_64_32 (out:W8.t Array64.t, offset:W64.t,
+                            in_0:W8.t Array32.t) : W8.t Array64.t * W64.t = {
     
     var i:W64.t;
     
@@ -1188,8 +1188,8 @@ module M(SC:Syscall_t) = {
     return (out, offset);
   }
   
-  proc __memcpy_u8u8_96_32 (out:W8.t Array96.t, offset:W64.t,
-                            in_0:W8.t Array32.t) : W8.t Array96.t * W64.t = {
+  proc __memcpy_u8u8_128_32 (out:W8.t Array128.t, offset:W64.t,
+                             in_0:W8.t Array32.t) : W8.t Array128.t * W64.t = {
     
     var i:W64.t;
     
@@ -1218,23 +1218,8 @@ module M(SC:Syscall_t) = {
     return (out, offset);
   }
   
-  proc __memcpy_u8u8_128_32 (out:W8.t Array128.t, offset:W64.t,
-                             in_0:W8.t Array32.t) : W8.t Array128.t * W64.t = {
-    
-    var i:W64.t;
-    
-    i <- (W64.of_int 0);
-    
-    while ((i \ult (W64.of_int 32))) {
-      out.[(W64.to_uint offset)] <- in_0.[(W64.to_uint i)];
-      i <- (i + (W64.of_int 1));
-      offset <- (offset + (W64.of_int 1));
-    }
-    return (out, offset);
-  }
-  
-  proc __memcpy_u8u8_64_32 (out:W8.t Array64.t, offset:W64.t,
-                            in_0:W8.t Array32.t) : W8.t Array64.t * W64.t = {
+  proc __memcpy_u8u8_96_32 (out:W8.t Array96.t, offset:W64.t,
+                            in_0:W8.t Array32.t) : W8.t Array96.t * W64.t = {
     
     var i:W64.t;
     
@@ -1263,6 +1248,21 @@ module M(SC:Syscall_t) = {
     return (out, offset);
   }
   
+  proc __memcpy_u8u8_32_32 (out:W8.t Array32.t, offset:W64.t,
+                            in_0:W8.t Array32.t) : W8.t Array32.t * W64.t = {
+    
+    var i:W64.t;
+    
+    i <- (W64.of_int 0);
+    
+    while ((i \ult (W64.of_int 32))) {
+      out.[(W64.to_uint offset)] <- in_0.[(W64.to_uint i)];
+      i <- (i + (W64.of_int 1));
+      offset <- (offset + (W64.of_int 1));
+    }
+    return (out, offset);
+  }
+  
   proc __memcpy_u8u8_2144_32 (out:W8.t Array2144.t, offset:W64.t,
                               in_0:W8.t Array32.t) : W8.t Array2144.t * W64.t = {
     
@@ -1278,30 +1278,12 @@ module M(SC:Syscall_t) = {
     return (out, offset);
   }
   
-  proc _memcpy_u8u8_32_32 (out:W8.t Array32.t, offset:W64.t,
-                           in_0:W8.t Array32.t) : W8.t Array32.t * W64.t = {
+  proc _memcpy_u8u8_64_32 (out:W8.t Array64.t, offset:W64.t,
+                           in_0:W8.t Array32.t) : W8.t Array64.t * W64.t = {
     
     
     
-    (out, offset) <@ __memcpy_u8u8_32_32 (out, offset, in_0);
-    return (out, offset);
-  }
-  
-  proc _memcpy_u8u8_96_32 (out:W8.t Array96.t, offset:W64.t,
-                           in_0:W8.t Array32.t) : W8.t Array96.t * W64.t = {
-    
-    
-    
-    (out, offset) <@ __memcpy_u8u8_96_32 (out, offset, in_0);
-    return (out, offset);
-  }
-  
-  proc _memcpy_u8u8_64_64 (out:W8.t Array64.t, offset:W64.t,
-                           in_0:W8.t Array64.t) : W8.t Array64.t * W64.t = {
-    
-    
-    
-    (out, offset) <@ __memcpy_u8u8_64_64 (out, offset, in_0);
+    (out, offset) <@ __memcpy_u8u8_64_32 (out, offset, in_0);
     return (out, offset);
   }
   
@@ -1314,12 +1296,21 @@ module M(SC:Syscall_t) = {
     return (out, offset);
   }
   
-  proc _memcpy_u8u8_64_32 (out:W8.t Array64.t, offset:W64.t,
-                           in_0:W8.t Array32.t) : W8.t Array64.t * W64.t = {
+  proc _memcpy_u8u8_64_64 (out:W8.t Array64.t, offset:W64.t,
+                           in_0:W8.t Array64.t) : W8.t Array64.t * W64.t = {
     
     
     
-    (out, offset) <@ __memcpy_u8u8_64_32 (out, offset, in_0);
+    (out, offset) <@ __memcpy_u8u8_64_64 (out, offset, in_0);
+    return (out, offset);
+  }
+  
+  proc _memcpy_u8u8_96_32 (out:W8.t Array96.t, offset:W64.t,
+                           in_0:W8.t Array32.t) : W8.t Array96.t * W64.t = {
+    
+    
+    
+    (out, offset) <@ __memcpy_u8u8_96_32 (out, offset, in_0);
     return (out, offset);
   }
   
@@ -1332,43 +1323,24 @@ module M(SC:Syscall_t) = {
     return (out, offset);
   }
   
-  proc _x_memcpy_u8u8_32_32 (out:W8.t Array32.t, offset:W64.t,
-                             in_0:W8.t Array32.t) : W8.t Array32.t * W64.t = {
+  proc _memcpy_u8u8_32_32 (out:W8.t Array32.t, offset:W64.t,
+                           in_0:W8.t Array32.t) : W8.t Array32.t * W64.t = {
     
     
     
-    out <- out;
-    offset <- offset;
-    in_0 <- in_0;
-    (out, offset) <@ _memcpy_u8u8_32_32 (out, offset, in_0);
-    out <- out;
-    offset <- offset;
+    (out, offset) <@ __memcpy_u8u8_32_32 (out, offset, in_0);
     return (out, offset);
   }
   
-  proc _x_memcpy_u8u8_96_32 (out:W8.t Array96.t, offset:W64.t,
-                             in_0:W8.t Array32.t) : W8.t Array96.t * W64.t = {
+  proc _x_memcpy_u8u8_64_32 (out:W8.t Array64.t, offset:W64.t,
+                             in_0:W8.t Array32.t) : W8.t Array64.t * W64.t = {
     
     
     
     out <- out;
     offset <- offset;
     in_0 <- in_0;
-    (out, offset) <@ _memcpy_u8u8_96_32 (out, offset, in_0);
-    out <- out;
-    offset <- offset;
-    return (out, offset);
-  }
-  
-  proc _x_memcpy_u8u8_64_64 (out:W8.t Array64.t, offset:W64.t,
-                             in_0:W8.t Array64.t) : W8.t Array64.t * W64.t = {
-    
-    
-    
-    out <- out;
-    offset <- offset;
-    in_0 <- in_0;
-    (out, offset) <@ _memcpy_u8u8_64_64 (out, offset, in_0);
+    (out, offset) <@ _memcpy_u8u8_64_32 (out, offset, in_0);
     out <- out;
     offset <- offset;
     return (out, offset);
@@ -1388,15 +1360,29 @@ module M(SC:Syscall_t) = {
     return (out, offset);
   }
   
-  proc _x_memcpy_u8u8_64_32 (out:W8.t Array64.t, offset:W64.t,
-                             in_0:W8.t Array32.t) : W8.t Array64.t * W64.t = {
+  proc _x_memcpy_u8u8_64_64 (out:W8.t Array64.t, offset:W64.t,
+                             in_0:W8.t Array64.t) : W8.t Array64.t * W64.t = {
     
     
     
     out <- out;
     offset <- offset;
     in_0 <- in_0;
-    (out, offset) <@ _memcpy_u8u8_64_32 (out, offset, in_0);
+    (out, offset) <@ _memcpy_u8u8_64_64 (out, offset, in_0);
+    out <- out;
+    offset <- offset;
+    return (out, offset);
+  }
+  
+  proc _x_memcpy_u8u8_96_32 (out:W8.t Array96.t, offset:W64.t,
+                             in_0:W8.t Array32.t) : W8.t Array96.t * W64.t = {
+    
+    
+    
+    out <- out;
+    offset <- offset;
+    in_0 <- in_0;
+    (out, offset) <@ _memcpy_u8u8_96_32 (out, offset, in_0);
     out <- out;
     offset <- offset;
     return (out, offset);
@@ -1416,19 +1402,17 @@ module M(SC:Syscall_t) = {
     return (out, offset);
   }
   
-  proc __memcpy_u8u8p_32 (out:W8.t Array32.t, offset:W64.t, in_0:W64.t,
-                          inlen:W64.t) : W8.t Array32.t * W64.t = {
+  proc _x_memcpy_u8u8_32_32 (out:W8.t Array32.t, offset:W64.t,
+                             in_0:W8.t Array32.t) : W8.t Array32.t * W64.t = {
     
-    var i:W64.t;
     
-    i <- (W64.of_int 0);
     
-    while ((i \ult inlen)) {
-      out.[(W64.to_uint offset)] <-
-      (loadW8 Glob.mem (W64.to_uint (in_0 + i)));
-      i <- (i + (W64.of_int 1));
-      offset <- (offset + (W64.of_int 1));
-    }
+    out <- out;
+    offset <- offset;
+    in_0 <- in_0;
+    (out, offset) <@ _memcpy_u8u8_32_32 (out, offset, in_0);
+    out <- out;
+    offset <- offset;
     return (out, offset);
   }
   
@@ -1448,12 +1432,19 @@ module M(SC:Syscall_t) = {
     return (out, offset);
   }
   
-  proc _memcpy_u8u8p_32 (out:W8.t Array32.t, offset:W64.t, in_0:W64.t,
-                         inlen:W64.t) : W8.t Array32.t * W64.t = {
+  proc __memcpy_u8u8p_32 (out:W8.t Array32.t, offset:W64.t, in_0:W64.t,
+                          inlen:W64.t) : W8.t Array32.t * W64.t = {
     
+    var i:W64.t;
     
+    i <- (W64.of_int 0);
     
-    (out, offset) <@ __memcpy_u8u8p_32 (out, offset, in_0, inlen);
+    while ((i \ult inlen)) {
+      out.[(W64.to_uint offset)] <-
+      (loadW8 Glob.mem (W64.to_uint (in_0 + i)));
+      i <- (i + (W64.of_int 1));
+      offset <- (offset + (W64.of_int 1));
+    }
     return (out, offset);
   }
   
@@ -1466,17 +1457,12 @@ module M(SC:Syscall_t) = {
     return (out, offset);
   }
   
-  proc _x_memcpy_u8u8p_32 (out:W8.t Array32.t, offset:W64.t, in_0:W64.t,
-                           inlen:W64.t) : W8.t Array32.t * W64.t = {
+  proc _memcpy_u8u8p_32 (out:W8.t Array32.t, offset:W64.t, in_0:W64.t,
+                         inlen:W64.t) : W8.t Array32.t * W64.t = {
     
     
     
-    out <- out;
-    offset <- offset;
-    in_0 <- in_0;
-    (out, offset) <@ _memcpy_u8u8p_32 (out, offset, in_0, inlen);
-    out <- out;
-    offset <- offset;
+    (out, offset) <@ __memcpy_u8u8p_32 (out, offset, in_0, inlen);
     return (out, offset);
   }
   
@@ -1494,8 +1480,22 @@ module M(SC:Syscall_t) = {
     return (out, offset);
   }
   
-  proc __memcpy_u8u8_2_64_2144 (out:W8.t Array64.t, in_0:W8.t Array2144.t,
-                                in_offset:W64.t, bytes:W64.t) : W8.t Array64.t *
+  proc _x_memcpy_u8u8p_32 (out:W8.t Array32.t, offset:W64.t, in_0:W64.t,
+                           inlen:W64.t) : W8.t Array32.t * W64.t = {
+    
+    
+    
+    out <- out;
+    offset <- offset;
+    in_0 <- in_0;
+    (out, offset) <@ _memcpy_u8u8p_32 (out, offset, in_0, inlen);
+    out <- out;
+    offset <- offset;
+    return (out, offset);
+  }
+  
+  proc __memcpy_u8u8_2_32_2144 (out:W8.t Array32.t, in_0:W8.t Array2144.t,
+                                in_offset:W64.t, bytes:W64.t) : W8.t Array32.t *
                                                                 W64.t = {
     
     var i:W64.t;
@@ -1510,8 +1510,8 @@ module M(SC:Syscall_t) = {
     return (out, in_offset);
   }
   
-  proc __memcpy_u8u8_2_32_2144 (out:W8.t Array32.t, in_0:W8.t Array2144.t,
-                                in_offset:W64.t, bytes:W64.t) : W8.t Array32.t *
+  proc __memcpy_u8u8_2_64_2144 (out:W8.t Array64.t, in_0:W8.t Array2144.t,
+                                in_offset:W64.t, bytes:W64.t) : W8.t Array64.t *
                                                                 W64.t = {
     
     var i:W64.t;
